Update CPI counts, comparison for find_in_array

timing/.Makefile.d
@@ -10,12 +10,6 @@ memsolve.vos memsolve.vok memsolve.required_vos: memsolve.v riscvTiming.vos
 examples/FreeRTOS/RTOSDemo_NoAsserts_Clz.vo examples/FreeRTOS/RTOSDemo_NoAsserts_Clz.glob examples/FreeRTOS/RTOSDemo_NoAsserts_Clz.v.beautified examples/FreeRTOS/RTOSDemo_NoAsserts_Clz.required_vo: examples/FreeRTOS/RTOSDemo_NoAsserts_Clz.v 
 examples/FreeRTOS/RTOSDemo_NoAsserts_Clz.vio: examples/FreeRTOS/RTOSDemo_NoAsserts_Clz.v 
 examples/FreeRTOS/RTOSDemo_NoAsserts_Clz.vos examples/FreeRTOS/RTOSDemo_NoAsserts_Clz.vok examples/FreeRTOS/RTOSDemo_NoAsserts_Clz.required_vos: examples/FreeRTOS/RTOSDemo_NoAsserts_Clz.v 
-examples/data_structures/array.vo examples/data_structures/array.glob examples/data_structures/array.v.beautified examples/data_structures/array.required_vo: examples/data_structures/array.v ../Picinae_riscv.vo
-examples/data_structures/array.vio: examples/data_structures/array.v ../Picinae_riscv.vio
-examples/data_structures/array.vos examples/data_structures/array.vok examples/data_structures/array.required_vos: examples/data_structures/array.v ../Picinae_riscv.vos
-examples/data_structures/array_opt.vo examples/data_structures/array_opt.glob examples/data_structures/array_opt.v.beautified examples/data_structures/array_opt.required_vo: examples/data_structures/array_opt.v ../Picinae_riscv.vo
-examples/data_structures/array_opt.vio: examples/data_structures/array_opt.v ../Picinae_riscv.vio
-examples/data_structures/array_opt.vos examples/data_structures/array_opt.vok examples/data_structures/array_opt.required_vos: examples/data_structures/array_opt.v ../Picinae_riscv.vos
-examples/data_structures/linked_list.vo examples/data_structures/linked_list.glob examples/data_structures/linked_list.v.beautified examples/data_structures/linked_list.required_vo: examples/data_structures/linked_list.v ../Picinae_riscv.vo
-examples/data_structures/linked_list.vio: examples/data_structures/linked_list.v ../Picinae_riscv.vio
-examples/data_structures/linked_list.vos examples/data_structures/linked_list.vok examples/data_structures/linked_list.required_vos: examples/data_structures/linked_list.v ../Picinae_riscv.vos
+examples/data_structures/array/find_in_array/array.vo examples/data_structures/array/find_in_array/array.glob examples/data_structures/array/find_in_array/array.v.beautified examples/data_structures/array/find_in_array/array.required_vo: examples/data_structures/array/find_in_array/array.v ../Picinae_riscv.vo
+examples/data_structures/array/find_in_array/array.vio: examples/data_structures/array/find_in_array/array.v ../Picinae_riscv.vio
+examples/data_structures/array/find_in_array/array.vos examples/data_structures/array/find_in_array/array.vok examples/data_structures/array/find_in_array/array.required_vos: examples/data_structures/array/find_in_array/array.v ../Picinae_riscv.vos
