timing/examples/data_structures/array/find_in_array/binary/find_in_array.h
@@ -1,0 +1,3 @@
+#include "../../../timing_experiments.h"
+
+uint32_t find_in_array(uint32_t* arr, uint32_t key, uint32_t size);
