timing/examples/data_structures/array_opt/binary/array_opt.c
@@ -1,4 +1,4 @@
-#include <stdint.h>
+#include "array_opt.h"
 
 uint32_t find_in_array(uint32_t* arr, uint32_t key, uint32_t size) {
     uint32_t i = 0;
@@ -10,5 +10,3 @@ uint32_t find_in_array(uint32_t* arr, uint32_t key, uint32_t size) {
 
     return i;
 }
-
-int main() {}
