timing/examples/data_structures/array_opt/binary/array_opt.h
@@ -1,0 +1,2 @@
+#include <stdint.h>
+uint32_t find_in_array(uint32_t* arr, uint32_t key, uint32_t size);
