timing/examples/data_structures/array_opt/binary/main.c
@@ -1,0 +1,37 @@
+#include "../../timing_experiments.h"
+#include "array_opt.h"
+
+int main() {
+    neorv32_rte_setup();
+    neorv32_uart0_setup(BAUD_RATE, 0);
+
+    srand(42);
+
+    for (uint32_t len = 1; len <= 100; ++len) {
+        uint32_t array[100];
+        for (uint32_t i = 0; i < len; i++)
+            array[i] = rand();
+
+        int insert_index = -1;
+        uint32_t key = rand();
+        if (rand() % 2) {
+            insert_index = rand() % len;
+            array[insert_index] = key;
+        }
+
+	START_TIMER;
+        uint32_t result = find_in_array(array, key, len);
+        PRINT_TIMER;
+
+        char str[128];
+        puts("Len: "); itoa(len, str, 10); puts(str);
+        puts(", key: "); itoa(key, str, 10); puts(str);
+        puts(result < len ? " found" : " not found\n");
+	if (result < len) {
+	        puts(" at index "); itoa(result, str, 10); puts(str); puts("\n");
+	}
+    }
+
+    return 0;
+}
+
