timing/examples/data_structures/timing_experiments.h
@@ -1,0 +1,21 @@
+#include <stdint.h>
+#include <stdio.h>
+#include <neorv32.h>
+
+#define BAUD_RATE 19200
+#define puts neorv32_uart0_puts
+
+#define START_TIMER \
+	{ neorv32_cpu_csr_write(CSR_MCYCLE, 0); }
+
+#define PRINT_TIMER { \
+	uint32_t cycles_low = neorv32_cpu_csr_read(CSR_MCYCLE); \
+	uint32_t cycles_high = neorv32_cpu_csr_read(CSR_MCYCLEH); \
+	uint64_t cycles = ((uint64_t)cycles_high << 32) | cycles_low; \
+	char cycles_str[128]; \
+	itoa(cycles, cycles_str, 10); \
+	puts("Cycle count read: "); \
+	puts(cycles_str); \
+	puts("\n"); \
+	neorv32_cpu_csr_write(CSR_MCYCLE, cycles); \
+}
